pulse/lib/steel/pulse/Pulse.Checker.Auto.Framing.fsti
@@ -1,3 +1,0 @@
-module Pulse.Checker.Auto.Framing
-open Pulse.Checker.Auto.Util
-// val step_match : prover_step_t
