pulse/lib/steel/pulse/Pulse.Prover.Common.fsti
@@ -1,0 +1,90 @@
+module Pulse.Prover.Common
+
+module T = FStar.Tactics
+
+open Pulse.Syntax
+open Pulse.Typing
+open Pulse.Checker.Common
+open Pulse.Typing.Metatheory
+open Pulse.Checker.VPropEquiv
+open Pulse.Prover.Util
+
+module T = FStar.Tactics
+
+module Psubst = Pulse.Prover.Substs
+
+let vprop_typing (g:env) (t:term) = tot_typing g t Tm_VProp
+
+noeq
+type preamble = {
+  g0 : env;
+
+  ctxt : vprop;
+  ctxt_typing : vprop_typing g0 ctxt;
+
+  t : st_term;
+  c : comp_st;
+
+  uvs : uvs:env { disjoint uvs g0 }
+}
+
+let pst_env (#g0:env) (uvs:env { disjoint uvs g0 }) (ss:Psubst.t g0) =
+  push_env g0 (psubst_env (filter_ss uvs ss) ss)
+
+noeq
+type prover_state (preamble:preamble) = {
+  ss : ss:Psubst.t preamble.g0 {
+    well_typed_ss preamble.uvs ss
+  };
+
+  solved_goals : term;
+
+  unsolved_goals : list term;
+
+  remaining_ctxt : list term;
+
+  steps : st_term;
+
+  t_typing
+    : st_typing (pst_env preamble.uvs ss)
+                (Psubst.subst_st_term ss preamble.t)
+                (Psubst.subst_comp ss preamble.c);
+
+  unsolved_goals_typing
+    : vprop_typing (pst_env preamble.uvs ss)
+                   (list_as_vprop unsolved_goals);
+
+  remaining_ctxt_typing
+    : vprop_typing preamble.g0 (list_as_vprop remaining_ctxt);
+  
+  steps_typing
+    : st_typing (pst_env preamble.uvs ss)
+                steps
+                (ghost_comp
+                   preamble.ctxt
+                   (Tm_Star (list_as_vprop remaining_ctxt) solved_goals));
+
+  c_pre_inv
+    : vprop_equiv (pst_env preamble.uvs ss)
+                  (Psubst.subst_term ss (comp_pre preamble.c))
+                  (Tm_Star (list_as_vprop unsolved_goals) solved_goals);
+
+  solved_goals_closed : squash (freevars solved_goals `Set.subset`
+                                dom preamble.g0);
+}
+
+let pst_extends (#preamble:_) (p1 p2:prover_state preamble) =
+  p1.ss `Psubst.subst_extends` p2.ss
+
+type prover_t =
+  #preamble:_ ->
+  p:prover_state preamble ->
+  T.Tac (option (p':prover_state preamble { p' `pst_extends` p /\
+                                            p'.unsolved_goals == [] }))
+
+type prover_step_t =
+  #preamble:_ ->
+  p:prover_state preamble ->
+  prover:prover_t ->
+  T.Tac (option (p':prover_state preamble { p' `pst_extends` p }))
+
