pulse/lib/steel/pulse/Pulse.Prover.fsti
@@ -1,0 +1,21 @@
+module Pulse.Prover
+
+module T = FStar.Tactics
+
+open Pulse.Syntax
+open Pulse.Typing
+open Pulse.Checker.Common
+open Pulse.Typing.Metatheory
+open Pulse.Checker.VPropEquiv
+open Pulse.Prover.Util
+open Pulse.Prover.Common
+
+val prover : prover_t
+
+val prove_precondition (#g:env) (#ctxt:term)
+  (ctxt_typing:vprop_typing g ctxt)
+  (#t:st_term) (#c:comp_st)
+  (t_typing:st_typing g t c)
+  : T.Tac (option (t:st_term &
+                   c:comp_st { comp_pre c == ctxt } &
+                   st_typing g t c))
